src/spec/TLS13.ConnectionState.ProtectedWireLemmas.fsti
@@ -448,6 +448,64 @@ val lemma_step_opposite_network_events_preserve_write_read_record_material_align
         write_read_record_material_aligned sender receiver)
       (ensures write_read_record_material_aligned sender_after receiver_after)
 
+val lemma_server_handshake_write_client_handshake_read_install_aligned
+  (server:CS.connection_model)
+  (client:CS.connection_model)
+  (material:CS.traffic_key_material)
+  (server_after:CS.connection_model)
+  (client_after:CS.connection_model)
+  : Lemma
+      (requires
+        CS.step_model
+          server
+          (CS.ConnLocalEvent
+            (CS.LocalInstallTrafficKeysForRole {
+              CS.install_role = CS.ServerEndpoint;
+              CS.install_payload = {
+                CS.install_epoch = CS.TrafficHandshake;
+                CS.install_direction = CS.TrafficWrite;
+                CS.install_material = material;
+              };
+            })) == Some server_after /\
+        CS.step_model
+          client
+          (CS.ConnLocalEvent
+            (CS.LocalInstallTrafficKeys {
+              CS.install_epoch = CS.TrafficHandshake;
+              CS.install_direction = CS.TrafficRead;
+              CS.install_material = material;
+            })) == Some client_after)
+      (ensures write_read_record_material_aligned server_after client_after)
+
+val lemma_client_handshake_write_server_handshake_read_install_aligned
+  (client:CS.connection_model)
+  (server:CS.connection_model)
+  (material:CS.traffic_key_material)
+  (client_after:CS.connection_model)
+  (server_after:CS.connection_model)
+  : Lemma
+      (requires
+        CS.step_model
+          client
+          (CS.ConnLocalEvent
+            (CS.LocalInstallTrafficKeys {
+              CS.install_epoch = CS.TrafficHandshake;
+              CS.install_direction = CS.TrafficWrite;
+              CS.install_material = material;
+            })) == Some client_after /\
+        CS.step_model
+          server
+          (CS.ConnLocalEvent
+            (CS.LocalInstallTrafficKeysForRole {
+              CS.install_role = CS.ServerEndpoint;
+              CS.install_payload = {
+                CS.install_epoch = CS.TrafficHandshake;
+                CS.install_direction = CS.TrafficRead;
+                CS.install_material = material;
+              };
+            })) == Some server_after)
+      (ensures write_read_record_material_aligned client_after server_after)
+
 val lemma_sent_replay_skip_empty_head_preserves_peer_stream
   (sender:CS.connection_model)
   (ev:CS.conn_event)
